%! Author = sebash
%! Date = 6/30/22

\documentclass{article}
\usepackage{blindtext}
\usepackage{amsmath, amssymb}
\usepackage[makeroom]{cancel}
\usepackage{pgfplots}
\usepgfplotslibrary{fillbetween}
\usepackage{tikz}
\usetikzlibrary{calc,shapes, arrows}
\usepackage{sectsty}
\usepackage{amssymb}


\newcommand{\tikzmark}[1]{\tikz[overlay,remember picture] \node (#1) {};}
\newcommand{\DrawBox}[2]{%
    \begin{tikzpicture}[overlay,remember picture]
        \draw[->,shorten >=5pt,shorten <=5pt,out=70,in=130,distance=0.5cm,#1] (MarkA.north) to (MarkC.north);
        \draw[->,shorten >=5pt,shorten <=5pt,out=50,in=140,distance=0.3cm,#2] (MarkA.north) to (MarkB.north);
    \end{tikzpicture}
}

\newcommand{\DrawBoxThree}[3]{%
    \begin{tikzpicture}[overlay,remember picture]
        \draw[->,shorten >=5pt,shorten <=5pt,out=70,in=130,distance=0.5cm,#1] (MarkA.north) to (MarkC.north);
        \draw[->,shorten >=5pt,shorten <=5pt,out=50,in=140,distance=0.3cm,#2] (MarkA.north) to (MarkB.north);
        \draw[->,shorten >=5pt,shorten <=5pt,out=90,in=120,distance=0.7cm,#3] (MarkA.north) to (MarkD.north);
    \end{tikzpicture}
}
\title{Sebastian Campos Homework}

\DeclareMathSizes{12}{30}{16}{12}

\begin{document}
    \maketitle
    \noindent
    \section*{10.1  1 to 25 odd}
    \subsection*{1 a}
    \begin{align*}
        (f \circ g)(x)
    \end{align*}
    \begin{align*}
        f(x) &= 4x + 3 &g(x) &= 2x +5
    \end{align*}
    \begin{align*}
        (f \circ g)(x) &= 4(2x + 5) + 3\\
        (f \circ g)(x) &= 8x + 20 + 3\\
        (f \circ g)(x) &= 8x + 23
    \end{align*}
    \begin{align*}
        \boxed{(f \circ g)(x) = 8x + 23}
    \end{align*}

    \subsection*{1 b}
    \begin{align*}
    (g \circ f)(x)
    \end{align*}
    \begin{align*}
        f(x) &= 4x + 3 &g(x) &= 2x +5
    \end{align*}
    \begin{align*}
        (g \circ f)(x) &= 2(4x + 3) + 5\\
        (g \circ f)(x) &= 8x + 6 + 5\\
        (g \circ f)(x) &= 8x + 11
    \end{align*}
    \begin{align*}
        \boxed{(g \circ f)(x) = 8x + 11}
    \end{align*}

    \subsection*{3 a}
    \begin{align*}
    (f \circ g)(x)
    \end{align*}
    \begin{align*}
        f(x) &= 6x -5  &g(x) &= 4x +1
    \end{align*}
    \begin{align*}
    (f \circ g)(x) &= 6(4x + 1) -5\\
    (f \circ g)(x) &= 24x + 6 - 5\\
    (f \circ g)(x) &= 24x + 1
    \end{align*}
    \begin{align*}
        \boxed{(f \circ g)(x) = 24x + 1}
    \end{align*}

    \subsection*{3 b}
    \begin{align*}
    (g \circ f)(x)
    \end{align*}
    \begin{align*}
        f(x) &= 6x -5  &g(x) &= 4x +1
    \end{align*}
    \begin{align*}
    (g \circ f)(x) &= 4(6x -5) +1\\
    (g \circ f)(x) &= 24x -20 +1 \\
    (g \circ f)(x) &= 24x -19
    \end{align*}
    \begin{align*}
        \boxed{(g \circ f)(x) = 24x -19}
    \end{align*}

    \subsection*{5 a}
    \begin{align*}
    (f \circ g)(x)
    \end{align*}
    \begin{align*}
        f(x) &= 3x  &g(x) &= 2x^2 - 3x
    \end{align*}
    \begin{align*}
    (f \circ g)(x) &= 3(2x^2 - 3x)\\
    (f \circ g)(x) &= 6x^2 - 9x\\
    \end{align*}
    \begin{align*}
        \boxed{(f \circ g)(x) = 6x^2 - 9x}
    \end{align*}

    \subsection*{5 b}
    \begin{align*}
    (g \circ f)(x)
    \end{align*}
    \begin{align*}
        f(x) &= 3x  &g(x) &= 2x^2 - 3x
    \end{align*}
    \begin{align*}
    (g \circ f)(x) &= 2(3x)^2 - 3(3x)\\
    (g \circ f)(x) &= 18x^2 - 9x \\
    \end{align*}
    \begin{align*}
        \boxed{(g \circ f)(x) = 18x^2 - 9x}
    \end{align*}

    \subsection*{7 a}
    \begin{align*}
    (f \circ g)(x)
    \end{align*}
    \begin{align*}
        f(x) &= 2x - 1  &g(x) &= x^2 + 2
    \end{align*}
    \begin{align*}
    (f \circ g)(x) &= 2(x^2 +2) - 1\\
    (f \circ g)(x) &= 2x^2 + 4 - 1\\
    (f \circ g)(x) &= 2x^2 + 3
    \end{align*}
    \begin{align*}
        \boxed{(f \circ g)(x) = 2x^2 + 3 }
    \end{align*}

    \subsection*{7 b}
    \begin{align*}
    (g \circ f)(x)
    \end{align*}
    \begin{align*}
        f(x) &= 2x - 1  &g(x) &= x^2 + 2
    \end{align*}
    \begin{align*}
    (g \circ f)(x) &= (2x - 1)^2 + 2\\
    (g \circ f)(x) &= (2x - 1)(2x - 1) + 2\\
    (g \circ f)(x) &= 4x^2 - 2x - 2x +1 + 2\\
    (g \circ f)(x) &= 4x^2 - 4x +3 \\
    \end{align*}
    \begin{align*}
        \boxed{(g \circ f)(x) = 4x^2 - 4x +3}
    \end{align*}



\end{document}